proof/agp32UpdateScript.sml
@@ -2326,6 +2326,29 @@ QED
 
 
 (* states exist to update specific items *)
+(** IF_instr **)
+Theorem agp32_IF_instr_exists_IF_instr_update:
+  !fext fbits t.
+    ?s s'. (agp32 fext fbits t).IF.IF_instr = (IF_instr_update (fext t) s s').IF.IF_instr
+Proof
+  rw [] >> Cases_on `t` >-
+   (rw [agp32_def,mk_module_def,mk_circuit_def] >>
+    clist_update_state_tac >>
+    fs [Abbr `s20`,Abbr `s19`,Abbr `s18`,Abbr `s17`,Abbr `s16`,Abbr `s15`,Abbr `s14`,
+      Abbr `s13`,Abbr `s12`,Abbr `s11`,Abbr `s10`,Abbr `s9`,Abbr `s8`,Abbr `s7`,
+      Abbr `s6`,Abbr `s5`,Abbr `s4`,
+      Hazard_ctrl_unchanged_IF,WB_update_unchanged_IF,MEM_imm_update_unchanged_IF,
+      MEM_ctrl_update_unchanged_IF,EX_data_rec_update_unchanged_IF,
+      EX_jump_sel_addr_update_unchanged_IF,EX_SHIFT_update_unchanged_IF,
+      EX_ALU_update_unchanged_IF,EX_compute_enable_update_unchanged_IF,
+      EX_ALU_input_update_unchanged_IF,EX_forward_data_unchanged_IF,
+      EX_ctrl_update_unchanged_IF,ID_data_update_unchanged_IF,
+      ID_imm_update_unchanged_IF,ID_opc_func_update_unchanged_IF,
+      IF_PC_input_update_def] >>
+    METIS_TAC []) >>
+  rw [agp32_IF_instr_updated_by_IF_instr_update]
+QED
+
 (** ID_opc and ID_func **)
 Theorem agp32_ID_opc_func_exists_ID_opc_func_update:
   !fext fbits t.
@@ -2392,74 +2415,6 @@ Proof
   qpat_abbrev_tac `s'' = mk_circuit (procs _) (procs _) (agp32_init fbits) fext t` >>
   qpat_abbrev_tac `s''' = procs _ (fext t) s'' s''` >>
   clist_update_state_tac >>  METIS_TAC []
-QED
-
-
-(** IF_PC_write_enable and EX_isAcc **)
-Theorem agp32_IF_PC_write_enable_and_EX_isAcc:
-  !fext fbits t.
-    (agp32 fext fbits t).IF.IF_PC_write_enable ==>
-    ~(agp32 fext fbits t).EX.EX_isAcc
-Proof
-  rw [] >> Cases_on `t` >>
-  fs [agp32_def,mk_module_def,mk_circuit_def] >-
-   (clist_update_state_tac >>
-    fs [Abbr `s20`,Hazard_ctrl_def] >>
-    Cases_on `s19.state = 3w \/ s19.state = 5w` >> fs [] >>
-    Cases_on `s19.state = 1w \/ s19.state = 2w \/ s19.state = 4w \/ s19.state = 6w` >> fs [] >>
-    Cases_on `(fext 0).ready` >> fs [] >>
-    Cases_on `(agp32_init fbits).MEM.MEM_opc = 2w \/ (agp32_init fbits).MEM.MEM_opc = 3w \/
-              (agp32_init fbits).MEM.MEM_opc = 4w \/ (agp32_init fbits).MEM.MEM_opc = 5w \/      
-              (agp32_init fbits).MEM.MEM_opc = 12w` >> fs [] >>
-    Cases_on `s19.EX.EX_isAcc` >> fs [] >>
-    Cases_on `s19.EX.EX_jump_sel` >> fs []) >>
-  qpat_abbrev_tac `s' = mk_circuit (procs _) (procs _) (agp32_init fbits) fext t` >>
-  qpat_abbrev_tac `s'' = procs _ (fext t) s' s'` >>
-  clist_update_state_tac >>
-  fs [Abbr `s20`,Hazard_ctrl_def] >>
-  Cases_on `s19.state = 3w \/ s19.state = 5w` >> fs [] >>
-  Cases_on `s19.state = 1w \/ s19.state = 2w \/ s19.state = 4w \/ s19.state = 6w` >> fs [] >>
-  Cases_on `(fext (SUC n)).ready` >> fs [] >>
-  Cases_on `s''.MEM.MEM_opc = 2w \/ s''.MEM.MEM_opc = 3w \/ s''.MEM.MEM_opc = 4w \/
-            s''.MEM.MEM_opc = 5w \/ s''.MEM.MEM_opc = 12w` >> fs [] >>
-  Cases_on `s19.EX.EX_isAcc` >> fs [] >>
-  Cases_on `s19.EX.EX_jump_sel` >> fs []      
-QED
-
-(** IF_PC_write_enable and state **)
-Theorem agp32_IF_PC_write_enable_and_state:
-  !fext fbits t.
-    (agp32 fext fbits t).IF.IF_PC_write_enable ==>
-    ((agp32 fext fbits t).state <> 1w) /\
-    ((agp32 fext fbits t).state <> 2w) /\
-    ((agp32 fext fbits t).state <> 3w) /\
-    ((agp32 fext fbits t).state <> 4w) /\
-    ((agp32 fext fbits t).state <> 5w) /\
-    ((agp32 fext fbits t).state <> 6w)
-Proof
-  rpt GEN_TAC >> STRIP_TAC >> Cases_on `t` >>
-  fs [agp32_def,mk_module_def,mk_circuit_def] >-
-   (clist_update_state_tac >>
-    fs [Abbr `s20`,Hazard_ctrl_def] >>
-    Cases_on `s19.state = 3w \/ s19.state = 5w` >> fs [] >>
-    Cases_on `s19.state = 1w \/ s19.state = 2w \/ s19.state = 4w \/ s19.state = 6w` >> fs [] >>
-    Cases_on `(fext 0).ready` >> fs [] >>
-    Cases_on `(agp32_init fbits).MEM.MEM_opc = 2w \/ (agp32_init fbits).MEM.MEM_opc = 3w \/
-              (agp32_init fbits).MEM.MEM_opc = 4w \/ (agp32_init fbits).MEM.MEM_opc = 5w \/      
-              (agp32_init fbits).MEM.MEM_opc = 12w` >> fs [] >>
-    Cases_on `s19.EX.EX_isAcc` >> fs [] >>
-    Cases_on `s19.EX.EX_jump_sel` >> fs []) >>
-  qpat_abbrev_tac `s' = mk_circuit (procs _) (procs _) (agp32_init fbits) fext t` >>
-  qpat_abbrev_tac `s'' = procs _ (fext t) s' s'` >>
-  clist_update_state_tac >>
-  fs [Abbr `s20`,Hazard_ctrl_def] >>
-  Cases_on `s19.state = 3w \/ s19.state = 5w` >> fs [] >>
-  Cases_on `s19.state = 1w \/ s19.state = 2w \/ s19.state = 4w \/ s19.state = 6w` >> fs [] >>
-  Cases_on `(fext (SUC n)).ready` >> fs [] >>
-  Cases_on `s''.MEM.MEM_opc = 2w \/ s''.MEM.MEM_opc = 3w \/ s''.MEM.MEM_opc = 4w \/
-            s''.MEM.MEM_opc = 5w \/ s''.MEM.MEM_opc = 12w` >> fs [] >>
-  Cases_on `s19.EX.EX_isAcc` >> fs [] >>
-  Cases_on `s19.EX.EX_jump_sel` >> fs []
 QED
 
 
